ver3_less_complex/Lemmas.dfy
@@ -6,18 +6,48 @@ module M_Lemma {
     import opened M_AuxilarilyFunc
 
     lemma{:axiom} Axiom_Byz_Constraints()
-    ensures |Adversary_Nodes| < f(|Honest_Nodes| + |Adversary_Nodes|)
+    ensures |Adversary_Nodes| <= f(|Honest_Nodes| + |Adversary_Nodes|)
     ensures Adversary_Nodes * Honest_Nodes == {}
+
+    lemma{:axiom} Axiom_Common_Constraints()
+    ensures All_Nodes != {}
+
+    lemma{:axiom} NoOuterClient()
+    ensures forall cert : Signature :: cert.signer in All_Nodes
 
     /**
      * Lemma: for 2 valid certificate, if they are not conflict, then their coressponding view number should be different
      */
     lemma LemmaViewDiffOnConflictCertificate(cert1 : Cert, cert2 : Cert)
     requires cert1.Cert? && cert2.Cert?
+    requires cert1.cType == cert2.cType
     requires ValidQC(cert1) && ValidQC(cert2)
+    requires cert1.block.Block? && cert2.block.Block?
     requires !NoConflict(cert1.block, cert2.block)
     ensures cert1.viewNum != cert2.viewNum
     {
+        var votesInCert1 := getVotesInValidQC(cert1);
+        var voterInCert1 := getMajoritySignerInValidQC(cert1);
 
+        var votesInCert2 := getVotesInValidQC(cert2);
+        var voterInCert2 := getMajoritySignerInValidQC(cert2);
+
+        // assert voterInCert1 <= All_Nodes && voterInCert2 <= All_Nodes;
+
+        // assert |Adversary_Nodes| <= f(|All_Nodes|);
+        assert |All_Nodes| > 0 by {
+            Axiom_Common_Constraints();
+        }
+
+        assert voterInCert1 * voterInCert2 * Honest_Nodes != {} by {
+            LemmaTwoQuorumIntersection(
+                All_Nodes,
+                Adversary_Nodes,
+                voterInCert1,
+                voterInCert2
+            );
+        }
     }
+
+
 }
