ver3_less_complex/common/sets.dfy
@@ -1,6 +1,7 @@
 
 
 module M_Set {
+
     method SetToSeq<T>(s: set<T>) returns (sq: seq<T>)
     ensures |sq| == |s| // The length of the sequence equals the size of the set
     ensures forall i :: 0 <= i < |sq| ==> sq[i] in s // All elements in the sequence are from the set
@@ -17,6 +18,28 @@ module M_Set {
             var x :| x in remaining;
             sq := sq + [x];
             remaining := remaining - {x};
+        }
+    }
+
+    lemma LemmaProperSubsetCardinality<T>(x: set<T>, y:set<T>)
+    requires x < y
+    ensures |x| < |y|
+    {
+        if (x != {}) {
+            var e :| e in x;
+            LemmaProperSubsetCardinality(x-{e}, y-{e});
+        }
+    }
+
+    lemma LemmaSubsetCardinality<T> (x: set<T>, y:set<T>)
+    ensures x < y ==> |x| < |y| // Strangely Dafny can't prove this. HAVE TO prove it by our own
+    ensures x <= y ==> |x| <= |y| 
+    {
+        if (x < y) {
+            LemmaProperSubsetCardinality(x, y);
+        }
+        if (x == y) {
+            // OBSERVE
         }
     }
 }
